Rename segment into fragment.

cfrontend/PrintCsyntax.ml
@@ -183,7 +183,7 @@ let print_pointer_hook
    : (formatter -> Values.block * Integers.Int.int -> unit) ref
    = ref (fun p (b, ofs) -> ())
 
-let print_pointer_seg_hook
+let print_pointer_frag_hook
    : (formatter -> Values.block * Integers.Int.int * Datatypes.nat -> unit) ref
    = ref (fun p (b, ofs, i) -> ())
 
@@ -201,8 +201,8 @@ let print_typed_value p v ty =
       fprintf p "%LdLL" (camlint64_of_coqint n)
   | Vptr(b, ofs), _ ->
       fprintf p "<ptr%a>" !print_pointer_hook (b, ofs)
-  | Vptrseg(b, ofs, i), _ ->
-      fprintf p "<ptrseg%a>" !print_pointer_seg_hook (b, ofs, i)
+  | Vptrfrag(b, ofs, i), _ ->
+      fprintf p "<ptrfrag%a>" !print_pointer_frag_hook (b, ofs, i)
   | Vundef, _ ->
       fprintf p "<undef>"
 
